@prefix ex: <http://example.org/> .
@prefix rdf: <http://www.w3.org/1999/02/22-rdf-syntax-ns#> .
@prefix rdfs: <http://www.w3.org/2000/01/rdf-schema#> .
@prefix owl: <http://www.w3.org/2002/07/owl#> .
@prefix xsd: <http://www.w3.org/2001/XMLSchema#> .
@prefix dc: <http://purl.org/dc/elements/1.1/> .
@prefix hed: <https://purl.org/hed#> .

<https://purl.org/hed> rdf:type owl:Ontology ;
    owl:versionInfo "1.0" ;
    rdfs:label "HED Base Schema Ontology" ;
    rdfs:comment "This is the base ontology." ;
    dc:title "HED Base Schema Ontology" ;
    dc:description "This ontology describes the base classes for the ontology." .

# Classes specifying the schema structure
hed:HedElement rdf:type owl:Class ;
    rdfs:comment "A class representing any object in a HED schema." .

#--------------------------------------------------------
# Specification of the schema sections

hed:HedSection rdf:type owl:Class ;
    rdfs:subClassOf hed:HedElement ;
    rdfs:comment "Represents the sections of the schema." ;
    rdfs:label "HedSection" .    

hed:HedHeaderSection rdf:type owl:Class ;
    rdfs:subClassOf hed:HedSection ;
    rdfs:comment "This section contains the schema header." ;
    rdfs:label "HedHeaderSection" ;   
    hed:wikiElementName "HED" ;
    hed:xmlElementName "HED" .

hed:HedPrologueSection rdf:type owl:Class ;
    rdfs:subClassOf hed:HedSection ;
    rdfs:comment "An overview of the schema and its purpose." ;
    rdfs:label "HedPrologueSection" ;   
    hed:wikiElementName "'''Prologue'''" ;
    hed:xmlElementName "prologue" .

hed:HedStartSchemaSection rdf:type owl:Class ;
    rdfs:subClassOf hed:HedSection ;
    rdfs:comment "The marker indicating the beginning of the main body of the schema." ;
    rdfs:label "HedStartSchemaSection" ;   
    hed:wikiElementName "!# start schema " ;
    hed:xmlElementName "schema" .

hed:HedEndSchemaSection rdf:type owl:Class ;
    rdfs:subClassOf hed:HedSection ;
    rdfs:comment "Required end marker for schema file." ;
    rdfs:label "HedEndSchemaSection" ;   
    hed:wikiElementName "!# end schema " ;
    hed:xmlElementName "/schema" .

hed:HedUnitClassesSection rdf:type owl:Class ;
    rdfs:subClassOf hed:HedSection ;
    rdfs:comment "Schema section defining unit classes and the units for the nodes." ;
    rdfs:label "HedUnitClassesSection" ;
    hed:wikiElementName "'''Unit classes'''" ;
    hed:xmlElementName "UnitClassDefinitions" .

hed:HedUnitModifiersSection rdf:type owl:Class ;
    rdfs:subClassOf hed:HedSection ;
    rdfs:comment "Schema section defining unit multiples and submultiples." ;
    rdfs:label "HedUnitModifiersSection" ;   
    hed:wikiElementName "'''Unit modifiers'''" ;
    hed:xmlElementName "UnitModifierDefinitions" .

hed:HedValueClassesSection rdf:type owl:Class ;
    rdfs:subClassOf hed:HedSection ;
    rdfs:comment "Schema section containing rules governing values provided for placeholders." ;
    rdfs:label "HedValueClassesSection" ;   
    hed:wikiElementName "'''Value classes'''" ;
    hed:xmlElementName "ValueClassDefinitions" .

hed:HedSchemaAttributesSection rdf:type owl:Class ;
    rdfs:subClassOf hed:HedSection ;
    rdfs:comment "Schema section defining the attribute modifiers of other sections of the schema." ;
    rdfs:label "HedSchemaAttributesSection" ;   
    hed:wikiElementName "'''Schema attributes'''" ;
    hed:xmlElementName "SchemaAttributeDefinitions" .

hed:HedPropertiesSection rdf:type owl:Class ;
    rdfs:subClassOf hed:HedSection ;
    rdfs:comment "Properties of the schema attributes themselves. These are used for schema handling and verification." ;
    rdfs:label "HedPropertiesSection" ;   
    hed:wikiElementName "'''Properties'''" ;
    hed:xmlElementName "PropertyDefinitions" .

hed:HedEpilogueSection rdf:type owl:Class ;
    rdfs:subClassOf hed:HedSection ;
    rdfs:comment "This section contains citation, licensing, and other information." ;
    rdfs:label "HedEpilogueSection" ;   
    hed:wikiElementName "'''Epilogue'''" ;
    hed:xmlElementName "epilogue" .

hed:HedEndSection rdf:type owl:Class ;
    rdfs:subClassOf hed:HedSection ;
    rdfs:comment "The required end marker for the HED schema." ;
    rdfs:label "HedEndSection" ;   
    hed:wikiElementName "!# end hed" ;
    hed:xmlElementName "/HED" .

# Hed tag class
hed:HedTag rdf:type owl:Class ;
    rdfs:subClassOf hed:HedElement ;
    rdfs:comment "Represents a HED term or node." ;
    rdfs:label "HedTag" ;
    hed:xmlElementName "node" .

# Hed tag placeholder class
hed:HedPlaceholder rdf:type owl:Class ;
    rdfs:subClassOf hed:HedTag ;
    rdfs:comment "Represents a node placeholder." ;
    rdfs:label "HedPlaceholder" .

hed:HedUnitClass rdf:type owl:Class ;
    rdfs:subClassOf hed:HedElement ;
    rdfs:comment "Organizes unit classes and the units for the nodes." ;
    rdfs:label "HedUnitClass" ;
    hed:wikiElementName "Unit classes" ;
    hed:xmlElementName "unitClassDefinitions" .

hed:HedUnit rdf:type owl:Class ;
    rdfs:subClassOf hed:HedElement ;
    rdfs:comment "Represents a unit element." ;
    rdfs:label "HedUnit" ;
    hed:xmlElementName "unit" ;
    hed:unitClass hed:HedUnitClass .

hed:HedUnitModifier rdf:type owl:Class ;
    rdfs:subClassOf hed:HedElement ;
    rdfs:comment "Organizes unit modifiers." ;
    rdfs:label "HedUnitModifier" ;
    hed:wikiElementName "Unit modifiers" ;
    hed:xmlElementName "unitModifierDefinitions" .


# '''Value classes''' <nowiki>[Specification of the rules for the values provided by users.]</nowiki>
hed:HedValueClass rdf:type owl:Class ;
    rdfs:subClassOf hed:HedElement ;
    rdfs:comment "The rules for the values provided by users." ;
    rdfs:label "HedValueClass" ;
    hed:wikiElementName "Value classes" ;
    hed:xmlElementName "valueClassDefinitions" .

# Properties pertaining to the structure of the schema.
hed:inSchemaSection rdf:type owl:ObjectProperty ;
    rdfs:comment "Indicates what section the element appears in." ;
    rdfs:label "inSchemaSection" ;
    rdfs:domain hed:HedElement ;
    rdfs:range hed:HedSection .    

hed:unitClass rdf:type owl:ObjectProperty ;
    rdfs:comment "Property specify the type of unit class a unit belongs to." ;
    rdfs:label "unitClass" ;
    rdfs:domain hed:HedUnit ;
    rdfs:range hed:HedUnitClass .


hed:wikiElementName rdf:type owl:DatatypeProperty ;
    rdfs:comment "The name of the element in MEDIAWIKI format." ;
    rdfs:label "wikiElementName" ;
    rdfs:domain hed:HedElement ;
    rdfs:range xsd:string .    

hed:xmlElementName rdf:type owl:DatatypeProperty ;
    rdfs:comment "The name of the element in XML format." ;
    rdfs:label "xmlElementName" ;
    rdfs:domain hed:HedElement ;
    rdfs:range xsd:string .  

hed:elementValue rdf:type owl:DatatypeProperty ;
    rdfs:comment "The value of an instance of the element." ;
    rdfs:label "elementValue" ;
    rdfs:domain hed:HedElement ;
    rdfs:range xsd:string .   


#--------------------------------------------------------
# Defining the Schema Header element

hed:library rdf:type owl:DatatypeProperty ;
    rdfs:comment "The name of the library schema if applicable." ;
    rdfs:label "library" ;
    hed:wikiElementName "library" ;
    hed:xmlElementName "library" ;            
    rdfs:domain hed:HedHeaderSection ;
    rdfs:range xsd:string .       

hed:unmerged rdf:type owl:DatatypeProperty ;
    rdfs:comment "If true, the schema is not merged with a partner schema." ;
    rdfs:label "unmerged" ;
    hed:wikiElementName "unmerged" ;
    hed:xmlElementName "unmerged" ;
    rdfs:domain hed:HedHeaderSection ;    
    rdfs:range xsd:boolean .     

hed:version rdf:type owl:DatatypeProperty ;
    rdfs:comment "The semantic version of this schema." ;
    rdfs:label "version" ;
    hed:wikiElementName "version" ;
    hed:xmlElementName "version" ;       
    rdfs:domain hed:HedHeaderSection ;    
    rdfs:range xsd:string .     

hed:withStandard rdf:type owl:DatatypeProperty ;
    rdfs:comment "The version of the schema's standard schema partner." ;
    rdfs:label "withStandard" ;
    hed:wikiElementName "withStandard" ;
    hed:xmlElementName "withStandard" ;               
    rdfs:domain hed:HedHeaderSection ;    
    rdfs:range xsd:string .


#------------------------------------------------------------------------------------
# * boolProperty <nowiki>[Indicates that the schema attribute represents something that is either true or false and does not have a value. Attributes without this value are assumed to have string values.]</nowiki>
hed:boolProperty rdf:type owl:AnnotationProperty ;
    rdfs:comment "This schema attribute represents something that is either true or false and does not have a value. Attributes without this value are assumed to have string values." ;
    rdfs:comment "Has an xsd:boolean value" ;        
    rdfs:label "boolProperty" ;
    hed:wikiElementName "Properties" ;
    hed:xmlElementName "propertyDefinitions" .

# * elementProperty <nowiki>[Indicates a schema attribute can apply to any type of element (tag term, unit class, etc).]</nowiki>
hed:elementProperty rdf:type owl:AnnotationProperty ;
    rdfs:comment "Indicates a schema attribute can apply to any type of element (tag term, unit class, etc)." ;
    rdfs:range xsd:boolean ;    
    rdfs:label "elementProperty" ;
    hed:wikiElementName "Properties" ;
    hed:xmlElementName "propertyDefinitions" .

# * isInheritedProperty <nowiki>[Indicates a schema attribute is inherited by child nodes. This property only applies to schema attributes for nodes.]</nowiki>
hed:isheritedProperty rdf:type owl:AnnotationProperty ;
    rdfs:comment "Indicates a schema attribute is inherited by child nodes. This property only applies to schema attributes for nodes." ;
    rdfs:range xsd:boolean ;   
    rdfs:label "isHeritedProperty" ;
    hed:wikiElementName "Properties" ;
    hed:xmlElementName "propertyDefinitions" .

# * nodeProperty <nowiki>[Indicates a attribute applies to node (tag-term) elements. This was added to allow for an attribute to apply to multiple elements.]</nowiki>
hed:nodeProperty rdf:type owl:AnnotationProperty ;
    rdfs:comment "Indicates a attribute applies to node (tag-term) elements. This was added to allow for an attribute to apply to multiple elements." ;
    rdfs:range xsd:boolean ;   
    rdfs:label "nodeProperty" ;
    hed:wikiElementName "Properties" ;
    hed:xmlElementName "propertyDefinitions" .

# * unitClassProperty <nowiki>[Indicates a schema attribute applies to unit classes.]</nowiki>
hed:unitClassProperty rdf:type owl:AnnotationProperty ;
    rdfs:comment "Indicates a schema attribute applies to unit classes." ;
    rdfs:range xsd:boolean ;      
    rdfs:label "unitClassProperty" ;
    hed:wikiElementName "Properties" ;
    hed:xmlElementName "propertyDefinitions" .

# * unitModifierProperty <nowiki>[Indicates a schema attribute applies to unit modifier classes.]</nowiki>
hed:unitModifierProperty rdf:type owl:AnnotationProperty ;
    rdfs:comment "Indicates a schema attribute applies to unit modifier classes." ;
    rdfs:range xsd:boolean ; 
    rdfs:label "unitModifierProperty" ;
    hed:wikiElementName "Properties" ;
    hed:xmlElementName "propertyDefinitions" .

# * unitProperty <nowiki>[Indicates that the schema attribute is meant to be applied to units within a unit class.]</nowiki> 
hed:unitProperty rdf:type owl:AnnotationProperty ;
    rdfs:comment "Indicates a schema attribute applies to units within a unit class." ;
    rdfs:range xsd:boolean ; 
    rdfs:label "unitProperty" ;
    hed:wikiElementName "Properties" ;
    hed:xmlElementName "propertyDefinitions" .

hed:valueClassProperty rdf:type owl:AnnotationProperty ;
    rdfs:comment "Indicates a schema attribute applies to value classes." ;
    rdfs:range xsd:boolean ;
    rdfs:label "valueClassProperty" ;
    hed:wikiElementName "Properties" ;
    hed:xmlElementName "propertyDefinitions" .

#------------------------------------------------------------------------------------
# Property definitions that are internal to the rdf representation of the HED schema
hed:hasHedParent rdf:type owl:ObjectProperty ;
    rdfs:comment "Represents the relationship of a HED term to its parent in HED hierarchy" ;
    rdfs:label "hasHedParent" ;
    rdfs:domain hed:HedTag ;
    rdfs:range hed:HedTag .   

# Property indicates that the Hed node is a top-level node in the HED schema
hed:isTopHedTag rdf:type owl:DatatypeProperty ;
    rdfs:comment "Indicates that the HedTag is a top-level tag." ;
    rdfs:label "isTopHedTag" ;
    rdfs:domain hed:HedTag ;
    rdfs:range xsd:boolean .    

#------------------------------------------------------------------------------------
# Schema attribute property definitions
hed:schemaAttributeDatatypeProperty rdf:type owl:DatatypeProperty .
hed:schemaAttributeObjectProperty rdf:type owl:ObjectProperty .        

# allowedCharacter
# * allowedCharacter <nowiki>{valueClassProperty}[A schema attribute of value classes specifying a special character that is allowed in expressing the value of a placeholder. Normally the allowed characters are listed individually. However, the word letters designates the upper and lower case alphabetic characters and the word digits designates the digits 0-9. The word blank designates the blank character.]</nowiki>
hed:allowedCharacter rdf:type owl:DatatypeProperty ;
    rdfs:subPropertyOf hed:schemaAttributeDatatypeProperty ;
    rdfs:comment "A schema attribute of value classes specifying a special character that is allowed in expressing the value of a placeholder. Normally the allowed characters are listed individually. However, the word letters designates the upper and lower case alphabetic characters and the word digits designates the digits 0-9. The word blank designates the blank character." ;
    rdfs:label "allowedCharacter" ;
    rdfs:domain hed:HedValueClass ;    
    rdfs:range xsd:string .

# conversionFactor
# * conversionFactor <nowiki>{unitProperty, unitModifierProperty}[The multiplicative factor to multiply these units to convert to default units.]</nowiki>
hed:conversionFactor rdf:type owl:DatatypeProperty ;
    rdfs:subPropertyOf hed:schemaAttributeDatatypeProperty ;
    rdfs:comment "The factor to multiply these units by to convert to default units." ;
    rdfs:label "conversionFactor" ;
    rdfs:domain hed:HedUnit ;
    rdfs:domain hed:HedUnitModifier ;    
    rdfs:range xsd:decimal .

# deprecatedFrom
# Note: this may change to an ObjectProperty if HedVersion is made a class
# * deprecatedFrom <nowiki>{elementProperty}[Indicates that this element is deprecated. The value of the attribute is the latest schema version in which the element appeared in undeprecated form.]</nowiki>                                                                                                                                                                                                                                                                                                                                                                                                                                                                                                                                                              # * deprecatedFrom <nowiki>{elementProperty}[Indicates that this element is deprecated. The value of the attribute is the latest schema version in which the element appeared in undeprecated form.]</nowiki>
hed:deprecatedFrom rdf:type owl:DatatypeProperty ;
    rdfs:subPropertyOf hed:schemaAttributeDatatypeProperty ;
    rdfs:comment "Indicates that this element is deprecated. The value of the attribute is the latest schema version in which the element appeared in undeprecated form." ;
    rdfs:label "deprecatedFrom" ;
    rdfs:domain hed:HedElement ;
    rdfs:range xsd:string .    

hed:defaultUnits rdf:type owl:ObjectProperty ;
    rdfs:subPropertyOf hed:schemaAttributeObjectProperty ;
    rdfs:comment "a top-level library schema node is identical to a node of the same name in the partnered standard schema. This attribute can only appear in nodes that have the inLibrary schema attribute." ;
    rdfs:label "defaultUnits" ;
    rdfs:domain hed:HedUnitClass ;
    rdfs:range hed:HedUnit .    

hed:extensionAllowed rdf:type owl:DatatypeProperty ;
    rdfs:subPropertyOf hed:schemaAttributeDatatypeProperty ;
    rdfs:comment "A schema attribute indicating that users can add unlimited levels of child nodes under this tag. This tag is propagated to child nodes with the exception of the hashtag placeholders." ;
    rdfs:label "extensionAllowed" ;
    rdfs:domain hed:HedTag ;
    rdfs:range xsd:boolean .    

# inLibrary
# Note: this may change to an owl:ObjectProperty if library becomes a class.
# * inLibrary <nowiki>{elementProperty} [Indicates this schema element came from the named library schema, not the standard schema. This attribute is added by tools when a library schema is merged into its partnered standard schema.]</nowiki>
hed:inLibrary rdf:type owl:DatatypeProperty ;
    rdfs:subPropertyOf hed:schemaAttributeDatatypeProperty ;
    rdfs:comment "Indicates this schema element came from the named library schema, not the standard schema. This attribute is added by tools when a library schema is merged into its partnered standard schema." ;
    rdfs:label "inLibrary" ;
    rdfs:domain hed:HedElement ;
    rdfs:range xsd:string .    

# recommended
# * recommended  <nowiki>{boolProperty, nodeProperty}[A schema attribute indicating that the event-level HED string should include this tag.]</nowiki> 
hed:recommended rdf:type owl:DatatypeProperty ;
    rdfs:subPropertyOf hed:schemaAttributeDatatypeProperty ;
    rdfs:comment "Indicates that the event-level HED string should include this tag." ;
    rdfs:label "recommended" ;
    rdfs:domain hed:HedTag ;
    rdfs:range xsd:boolean .    

# relatedTag
# * relatedTag <nowiki>{nodeProperty, isInheritedProperty}[A schema attribute suggesting HED tags that are closely related to this tag. This attribute is used by tagging tools.]</nowiki>
hed:relatedTag rdf:type owl:ObjectProperty ;
    rdfs:subPropertyOf hed:schemaAttributeObjectProperty ;
    rdfs:comment "Indicates another tag  that is closely related to this tag. This attribute is used by tagging tools to provide tagging suggestions" ;
    rdfs:label "relatedTag" ;
    rdfs:domain hed:HedTag ;
    rdfs:range hed:HedTag .    


# requireChild
# * requireChild  <nowiki>{boolProperty, nodeProperty}[A schema attribute indicating that one of the node elements descendants must be included when using this tag.]</nowiki> 
hed:requireChild rdf:type owl:DatatypeProperty ;
    rdfs:subPropertyOf hed:schemaAttributeDatatypeProperty ;
    rdfs:comment "Indicates that that one of the node's descendants must be included when using this tag." ;
    rdfs:label "requireChild" ;
    rdfs:domain hed:HedTag ;
    rdfs:range xsd:boolean .    

# required
# * required <nowiki>{boolProperty, nodeProperty}[A schema attribute indicating that every event-level HED string should include this tag.]</nowiki>
hed:required rdf:type owl:DatatypeProperty ;
    rdfs:subPropertyOf hed:schemaAttributeDatatypeProperty ;
    rdfs:comment "A schema attribute indicating that every event-level HED string should include this tag." ;
    rdfs:label "required" ;
    rdfs:domain hed:HedTag ;
    rdfs:range xsd:boolean .    

# reserved
# * reserved <nowiki>{boolProperty, nodeProperty}[A schema attribute indicating that this tag has special meaning and requires special handling by tools.]</nowiki>
hed:reserved rdf:type owl:DatatypeProperty ;
    rdfs:subPropertyOf hed:schemaAttributeDatatypeProperty ;
    rdfs:comment "Indicates that this tag has special meaning and requires special handling by tools." ;
    rdfs:label "reserved" ;
    rdfs:domain hed:HedTag ;
    rdfs:range xsd:boolean .    

# rooted
# * rooted <nowiki>{nodeProperty}[Indicates a top-level library schema node is identical to a node of the same name in the partnered standard schema. This attribute can only appear in nodes that have the inLibrary schema attribute.]</nowiki>
hed:rooted rdf:type owl:ObjectProperty ;
    rdfs:subPropertyOf hed:schemaAttributeObjectProperty ;
    rdfs:comment "Indicates that a top-level library schema node is identical to a node of the same name in the partnered standard schema. This attribute can only appear in nodes that have the inLibrary schema attribute." ;
    rdfs:label "rooted" ;
    rdfs:domain hed:HedTag ;
    rdfs:range hed:HedTag .    

# SIUnit
# * SIUnit  <nowiki>{boolProperty, unitProperty}[A schema attribute indicating that this unit element is an SI unit and can be modified by multiple and submultiple names. Note that some units such as byte are designated as SI units although they are not part of the standard.]</nowiki>
hed:SIUnit rdf:type owl:DatatypeProperty ;
    rdfs:subPropertyOf hed:schemaAttributeDatatypeProperty ;
    rdfs:comment "Indicates that this unit element is an SI unit and can be modified by multiple and submultiple names. Note that some units such as byte are designated as SI units although they are not part of the standard." ;
    rdfs:label "SIUnit" ;
    rdfs:domain hed:HedUnit ;
    rdfs:range xsd:boolean .    

# SIUnitModifier
# * SIUnitModifier <nowiki>{boolProperty, unitModifierProperty}[A schema attribute indicating that this SI unit modifier represents a multiple or submultiple of a base unit rather than a unit symbol.]</nowiki> 
hed:SIUnitModifier rdf:type owl:DatatypeProperty ;
    rdfs:subPropertyOf hed:schemaAttributeDatatypeProperty ;
    rdfs:comment "Indicates that this SI unit modifier represents a multiple or submultiple of a base unit rather than a unit symbol." ;
    rdfs:label "SIUnitModifier" ;
    rdfs:domain hed:HedUnitModifier ;
    rdfs:range xsd:boolean .    

# SIUnitSymbolModifier
# * SIUnitSymbolModifier <nowiki>{boolProperty, unitModifierProperty}[A schema attribute indicating that this SI unit modifier represents a multiple or submultiple of a unit symbol rather than a base symbol.]</nowiki>
hed:SIUnitSymbolModifier rdf:type owl:DatatypeProperty ;
    rdfs:subPropertyOf hed:schemaAttributeDatatypeProperty ;
    rdfs:comment "Indicates that this SI unit modifier represents a multiple or submultiple of a unit symbol rather than a base symbol." ;
    rdfs:label "SIUnitSymbolModifier" ;
    rdfs:domain hed:HedUnitModifier ;
    rdfs:range xsd:boolean .    

# suggestedTag
# * suggestedTag <nowiki>{nodeProperty, isInheritedProperty}[A schema attribute that indicates another tag  that is often associated with this tag. This attribute is used by tagging tools to provide tagging suggestions.]</nowiki>
hed:suggestedTag rdf:type owl:ObjectProperty ;
    rdfs:subPropertyOf hed:schemaAttributeObjectProperty ;
    rdfs:comment "Indicates another tag  that is often associated with this tag. This attribute is used by tagging tools to provide tagging suggestions" ;
    rdfs:label "suggestedTag" ;
    rdfs:domain hed:HedTag ;
    rdfs:range hed:HedTag .    

# tagGroup
# * tagGroup <nowiki>{boolProperty, nodeProperty}[A schema attribute indicating the tag can only appear inside a tag group.] </nowiki> 
hed:tagGroup rdf:type owl:DatatypeProperty ;
    rdfs:subPropertyOf hed:schemaAttributeDatatypeProperty ;
    rdfs:comment "Indicates that the tag can only appear inside a tag group." ;
    rdfs:label "tagGroup" ;
    rdfs:domain hed:HedTag ;
    rdfs:range xsd:boolean .    

# takesValue
# * takesValue <nowiki>{boolProperty, nodeProperty}[A schema attribute indicating the tag is a hashtag placeholder that is expected to be replaced with a user-defined value.] </nowiki> 
hed:takesValue rdf:type owl:DatatypeProperty ;
    rdfs:subPropertyOf hed:schemaAttributeDatatypeProperty ;
    rdfs:comment "Indicates that the tag is a hashtag placeholder that is expected to be replaced with a user-defined value." ;
    rdfs:label "takesValue" ;
    rdfs:domain hed:HedTag ;
    rdfs:range xsd:boolean .    

# topLevelTagGroup
# * topLevelTagGroup <nowiki>{boolProperty, nodeProperty}[A schema attribute indicating that this tag (or its descendants) can only appear in a top-level tag group. A tag group can have at most one tag with this attribute.] </nowiki>
hed:topLevelTagGroup rdf:type owl:DatatypeProperty ;
    rdfs:subPropertyOf hed:schemaAttributeDatatypeProperty ;
    rdfs:comment "Indicates that this tag (or its descendants) can only appear in a top-level tag group. A tag group can have at most one tag with this attribute." ;
    rdfs:label "topLevelTagGroup" ;
    rdfs:domain hed:HedTag ;
    rdfs:range xsd:boolean .    

# unique
# * unique <nowiki>{boolProperty, nodeProperty}[A schema attribute indicating that only one of this tag or its descendants can be used  in the event-level HED string.]</nowiki> 
hed:unique rdf:type owl:DatatypeProperty ;
    rdfs:subPropertyOf hed:schemaAttributeDatatypeProperty ;
    rdfs:comment "Indicates that only one of this tag or its descendants can be used in the event-level HED string." ;
    rdfs:label "unique" ;
    rdfs:domain hed:HedTag ;
    rdfs:range xsd:boolean .    

# unitClass
# * unitClass <nowiki>{nodeProperty}[A schema attribute specifying which unit class this value tag belongs to.]</nowiki> 
hed:unitClass rdf:type owl:ObjectProperty ;
    rdfs:subPropertyOf hed:schemaAttributeObjectProperty ;
    rdfs:comment "Indicates which unit class this value tag belongs to." ;
    rdfs:label "unitClass" ;
    rdfs:domain hed:HedTag ;
    rdfs:range hed:HedUnitClass .    

# unitPrefix
# * unitPrefix <nowiki>{boolProperty, unitProperty}[A schema attribute applied specifically to unit elements to designate that the unit indicator is a prefix (e.g., dollar sign in the currency units).]</nowiki> 
hed:unitPrefix rdf:type owl:DatatypeProperty ;
    rdfs:subPropertyOf hed:schemaAttributeDatatypeProperty ;
    rdfs:comment "Indicates a prefix (e.g., dollar sign in the currency units)." ;
    rdfs:label "unitPrefix" ;
    rdfs:domain hed:HedUnit ;
    rdfs:range xsd:boolean .    

# unitSymbol
# * unitSymbol <nowiki>{boolProperty, unitProperty}[A schema attribute indicating this tag is an abbreviation or symbol representing a type of unit. Unit symbols represent both the singular and the plural and thus cannot be pluralized.]</nowiki>
hed:unitSymbol rdf:type owl:DatatypeProperty ;
    rdfs:subPropertyOf hed:schemaAttributeDatatypeProperty ;
    rdfs:comment "Indicates that an abbreviation or symbol representing a type of unit. Unit symbols represent both the singular and the plural and thus cannot be pluralized." ;
    rdfs:label "unitSymbol" ;
    rdfs:domain hed:HedUnit ;
    rdfs:range xsd:boolean .    

# valueClass
# * valueClass <nowiki>{nodeProperty}[A schema attribute specifying which value class this value tag belongs to.]</nowiki> 
hed:valueClass rdf:type owl:ObjectProperty ;
    rdfs:subPropertyOf hed:schemaAttributeObjectProperty ;
    rdfs:comment "Indicates which value class this value tag belongs to." ;
    rdfs:label "valueClass" ;
    rdfs:domain hed:HedTag ;
    rdfs:range hed:HedValueClass .


## -----------------------------------------------------
# Custom data types
hed:LetterString rdf:type rdfs:Datatype ;
    owl:onDatatype xsd:string ;
    owl:withRestrictions ([ xsd:pattern "[a-zA-Z]+" ]) ;
    rdfs:comment "Represents values that are in letters" ;
    rdfs:label "letters" .

ex:CustomEmail rdf:type rdfs:Datatype ;
    owl:onDataType xsd:string ;
    owl:withRestrictions ([ xsd:pattern "[a-zA-Z0-9._%+-]+@[a-zA-Z0-9.-]+\\.[a-zA-Z]{2,4}" ]) .  

# --------------------------------------------------------------------------------------

